spec/machine/Time.thy
@@ -1,0 +1,257 @@
+(*
+ * Copyright 2026, Proofcraft Pty Ltd
+ *
+ * SPDX-License-Identifier: GPL-2.0-only
+ *)
+
+theory Time
+imports
+  Kernel_Config \<comment> \<open>currently unnecessary, but added in anticipation of future use\<close>
+  Eisbach_Tools.Eisbach_Methods
+begin
+
+consts maxTimer_us :: "64 word"
+consts max_ticks_to_us :: "64 word"
+consts max_us_to_ticks :: "64 word"
+
+type_synonym ticks_len = 64
+
+type_synonym ticks = "ticks_len word"
+type_synonym time  = "ticks_len word"
+
+abbreviation max_time :: time where
+  "max_time \<equiv> max_word"
+
+definition \<mu>s_in_ms :: "64 word" where
+  "\<mu>s_in_ms = 1000"
+
+text \<open> This matches @{text "60 * 60 * MS_IN_S * US_IN_MS"} because it should be in micro-seconds. \<close>
+definition MAX_PERIOD_US :: "64 word" where
+  "MAX_PERIOD_US \<equiv> 60 * 60 * 1000 * 1000"
+
+\<comment> \<open>The following notepad shows that the axioms introduced below, which provide various results
+    about several constants and their conversion via us_to_ticks, are consistent.\<close>
+
+notepad begin
+
+define ticks_per_timer_unit :: "64 word" where "ticks_per_timer_unit = of_nat 50"
+define timer_unit :: "64 word" where "timer_unit = of_nat 1"
+define kernelWCET_us :: "64 word" where "kernelWCET_us = of_nat 100"
+define us_to_ticks :: "64 word \<Rightarrow> 64 word" where
+  "us_to_ticks = (\<lambda>us. (us * ticks_per_timer_unit) div timer_unit)"
+
+have kernelWCET_us_pos2: "0 < 2 * kernelWCET_us"
+  by (simp add: kernelWCET_us_def)
+
+have MIN_BUDGET_le_MAX_PERIOD: "2 * kernelWCET_us \<le> MAX_PERIOD_US"
+  by (simp add: kernelWCET_us_def MAX_PERIOD_US_def)
+
+have ticks_per_timer_unit_non_zero: "ticks_per_timer_unit \<noteq> 0"
+  by (simp add: ticks_per_timer_unit_def)
+
+have MIN_BUDGET_bound: "2 * unat kernelWCET_us * unat ticks_per_timer_unit < unat max_time"
+  apply (subst unat_max_word[symmetric])
+  apply clarsimp
+  apply (prop_tac "unat kernelWCET_us \<le> 100")
+   apply (fastforce simp: kernelWCET_us_def)
+  apply (prop_tac "unat ticks_per_timer_unit \<le> 50")
+   apply (fastforce simp: ticks_per_timer_unit_def)
+  apply (rule_tac y="10000" in le_less_trans)
+   apply (rule_tac j1=200 and l1=50 in order.trans[OF mult_le_mono]; fastforce)
+  apply simp
+  done
+
+have getCurrentTime_buffer_bound:
+  "5 * unat MAX_PERIOD_US * unat ticks_per_timer_unit < unat max_time"
+  by (fastforce simp: unat_max_word[symmetric] ticks_per_timer_unit_def MAX_PERIOD_US_def)
+
+have kernelWCET_pos': "0 < us_to_ticks kernelWCET_us"
+  apply (clarsimp simp: us_to_ticks_def word_less_nat_alt)
+  apply (subst unat_mult_lem' | subst unat_div
+         | fastforce simp: kernelWCET_us_def ticks_per_timer_unit_def timer_unit_def unat_minus_one_word)+
+  done
+
+have MIN_BUDGET_pos': "0 < 2 * us_to_ticks kernelWCET_us"
+  apply (clarsimp simp: us_to_ticks_def word_less_nat_alt)
+  apply (subst unat_mult_lem' | subst unat_div
+         | fastforce simp: kernelWCET_us_def ticks_per_timer_unit_def timer_unit_def unat_minus_one_word)+
+  done
+
+have init_domain_time_pos: "0 < us_to_ticks (15 * \<mu>s_in_ms)"
+  apply (clarsimp simp: us_to_ticks_def word_less_nat_alt)
+  apply (subst unat_mult_lem' | subst unat_div
+         | fastforce simp: \<mu>s_in_ms_def ticks_per_timer_unit_def timer_unit_def unat_minus_one_word)+
+  done
+
+have init_domain_time_bound: "15 * unat \<mu>s_in_ms * unat ticks_per_timer_unit < unat max_time"
+  by (subst unat_mult_lem'
+      | fastforce simp: \<mu>s_in_ms_def ticks_per_timer_unit_def unat_minus_one_word)+
+
+have getCurrentTime_buffer_pos:
+  "0 < 5 * us_to_ticks MAX_PERIOD_US"
+  by (fastforce simp: us_to_ticks_def word_less_nat_alt MAX_PERIOD_US_def
+                      ticks_per_timer_unit_def timer_unit_def)
+
+end (* notepad *)
+
+consts kernelWCET_us :: ticks
+
+axiomatization where
+  kernelWCET_us_pos2: "0 < 2 * kernelWCET_us"
+and
+  MIN_BUDGET_le_MAX_PERIOD: "2 * kernelWCET_us \<le> MAX_PERIOD_US"
+
+consts ticks_per_timer_unit :: ticks
+consts timer_unit :: ticks
+
+definition
+  "us_to_ticks us = (us * ticks_per_timer_unit) div timer_unit"
+
+definition
+  "ticks_to_us ticks = ticks div (ticks_per_timer_unit div timer_unit)"
+
+axiomatization where
+  ticks_per_timer_unit_non_zero: "ticks_per_timer_unit \<noteq> 0"
+and
+  MIN_BUDGET_bound: "2 * unat kernelWCET_us * unat ticks_per_timer_unit < unat max_time"
+and
+  \<comment> \<open>the 5 is from time_buffer_const (defined below)\<close>
+  getCurrentTime_buffer_bound:
+    "5 * unat MAX_PERIOD_US * unat ticks_per_timer_unit < unat max_time"
+and
+  kernelWCET_pos': "0 < us_to_ticks kernelWCET_us"
+and
+  MIN_BUDGET_pos': "0 < 2 * us_to_ticks kernelWCET_us"
+and
+  \<comment> \<open>the 15 is from the domain time of the initial state\<close>
+  init_domain_time_pos: "0 < us_to_ticks (15 * \<mu>s_in_ms)"
+and
+  \<comment> \<open>the 15 is from the domain time of the initial state\<close>
+  init_domain_time_bound: "15 * unat \<mu>s_in_ms * unat ticks_per_timer_unit < unat max_time"
+and
+  \<comment> \<open>the 5 is from time_buffer_const (defined below)\<close>
+  getCurrentTime_buffer_pos: "0 < 5 * us_to_ticks MAX_PERIOD_US"
+
+definition "MAX_PERIOD = us_to_ticks MAX_PERIOD_US"
+
+lemma kernelWCET_us_pos:
+  "0 < kernelWCET_us"
+  using kernelWCET_us_pos2 double_eq_zero_iff word_greater_zero_iff by blast
+
+definition
+  "kernelWCET_ticks = us_to_ticks kernelWCET_us"
+
+text \<open>
+  It is crucial that time does not overflow, and that overflow does not occur when performing any
+  operation which modifies the refill lists. We therefore impose a cap on the time that can be
+  returned by getCurrentTime, namely getCurrentTime_buffer. This is chosen to be the greatest word
+  t such that if a refill list has its head r_time at t, and satisfies valid_refills, then
+  when performing any function which does modify the refill list, overflow does not occur. The
+  choice depends heavily on the implementation of refill_budget_check.
+ \<close>
+
+abbreviation time_buffer_const where "time_buffer_const \<equiv> 5"
+
+abbreviation (input) getCurrentTime_buffer where
+  "getCurrentTime_buffer \<equiv> time_buffer_const * MAX_PERIOD"
+
+lemma replicate_no_overflow:
+  "n * unat (a :: ticks) \<le> unat (upper_bound :: ticks)
+   \<Longrightarrow> unat (of_nat n * a) = n * unat a"
+  by (metis (mono_tags, opaque_lifting) le_unat_uoi of_nat_mult word_unat.Rep_inverse)
+
+lemma kernelWCET_ticks_pos2: "0 < 2 * kernelWCET_ticks"
+  apply (simp add: kernelWCET_ticks_def)
+  using MIN_BUDGET_pos' by simp
+
+lemma getCurrentTime_buffer_nonzero':
+  "0 < getCurrentTime_buffer"
+  apply (insert getCurrentTime_buffer_pos)
+  apply (clarsimp simp: kernelWCET_ticks_def MAX_PERIOD_def)
+  done
+
+lemma us_to_ticks_helper:
+  "unat a * unat ticks_per_timer_unit \<le> unat max_time
+   \<Longrightarrow> unat (us_to_ticks a) \<le> unat a * unat ticks_per_timer_unit"
+  apply (clarsimp simp: us_to_ticks_def)
+  apply (subst unat_div | subst unat_mult_lem' | simp)+
+  done
+
+lemma getCurrentTime_buffer_no_overflow:
+  "5 * unat MAX_PERIOD < unat max_time"
+  apply (insert getCurrentTime_buffer_bound)
+  apply (rule_tac y=" 5 * unat MAX_PERIOD_US * unat ticks_per_timer_unit" in le_less_trans;
+         fastforce intro: us_to_ticks_helper simp: MAX_PERIOD_def)
+  done
+
+lemma MAX_PERIOD_mult:
+  "(n :: 64 word) \<le> 5 \<Longrightarrow> unat (n * MAX_PERIOD) = unat n * unat MAX_PERIOD"
+  apply (insert getCurrentTime_buffer_bound)
+  apply (insert replicate_no_overflow[where n="unat n" and a=MAX_PERIOD and upper_bound=max_time, atomized])
+  apply (elim impE)
+   apply (clarsimp simp: MAX_PERIOD_def)
+   apply (prop_tac "unat n \<le> (5 :: nat)")
+    apply (clarsimp simp: word_le_nat_alt)
+   apply (prop_tac "unat (us_to_ticks MAX_PERIOD_US) \<le> unat MAX_PERIOD_US * unat ticks_per_timer_unit")
+  apply (simp add: us_to_ticks_helper)
+   apply (prop_tac "5 * (unat MAX_PERIOD_US * unat ticks_per_timer_unit) \<le> unat max_time")
+    apply linarith
+   apply (metis (no_types, opaque_lifting) le_trans mult.commute mult_le_mono1)
+  apply (metis word_unat.Rep_inverse)
+  done
+
+lemma getCurrentTime_buffer_no_overflow':
+  "5 * unat MAX_PERIOD = unat getCurrentTime_buffer"
+  apply (subst unat_mult_lem')
+   apply (metis MAX_PERIOD_mult add.left_neutral order_refl unat_plus_simple unat_sum_boundE
+                word_zero_le)
+  apply (fastforce simp: us_to_ticks_helper)
+  done
+
+lemma us_to_ticks_zero:
+  "us_to_ticks 0 = 0"
+  by (clarsimp simp: us_to_ticks_def)
+
+lemma unat_div_helper:
+  "a * ticks_per_timer_unit \<le> b * ticks_per_timer_unit
+   \<Longrightarrow> unat (a * ticks_per_timer_unit div timer_unit) \<le> unat (b * ticks_per_timer_unit div timer_unit)"
+  by (simp add: div_le_mono unat_div_distrib word_le_nat_alt)
+
+lemma us_to_ticks_mono:
+  "\<lbrakk>a \<le> b; unat b * unat ticks_per_timer_unit \<le> unat max_time\<rbrakk>
+    \<Longrightarrow> us_to_ticks a \<le> us_to_ticks b"
+  apply (simp add: us_to_ticks_def)
+  apply (clarsimp simp: word_le_nat_alt)
+  apply (rule unat_div_helper)
+  apply (clarsimp simp: word_le_nat_alt)
+  apply (metis (no_types, opaque_lifting) le_unat_uoi mult_le_mono1 word_arith_nat_defs(2))
+  done
+
+lemma divide_le_helper:
+  "\<lbrakk>unat a * unat b  \<le> unat (max_word :: 'a :: len word)\<rbrakk>
+   \<Longrightarrow> (a :: 'a :: len word) * (b  div c) \<le> a * b div c"
+  apply (clarsimp simp: word_le_nat_alt)
+  apply (subst unat_div | subst unat_mult_lem')+
+  apply (blast intro: div_le_dividend le_trans mult_le_mono2)
+  apply (subst unat_div | subst unat_mult_lem' | simp)+
+  apply (metis (no_types, opaque_lifting) Groups.mult_ac(3) arith_extra_simps(19) div_by_0
+                                          div_le_mono mult_le_mono2 nonzero_mult_div_cancel_left
+                                          thd)
+  done
+
+lemma MIN_BUDGET_helper:
+  "2 * us_to_ticks kernelWCET_us \<le> us_to_ticks (2 * kernelWCET_us)"
+  apply (clarsimp simp: us_to_ticks_def)
+  apply (insert MIN_BUDGET_bound)
+  apply (rule_tac order_trans[OF divide_le_helper])
+   apply (subst unat_mult_lem' | simp)+
+  apply (simp add: mult.assoc)
+  done
+
+definition "MAX_RELEASE_TIME = max_time - 5 * MAX_PERIOD"
+
+lemma unat_MAX_RELEASE_TIME:
+  "unat MAX_RELEASE_TIME = unat max_time - 5 * unat MAX_PERIOD"
+  by (clarsimp simp: MAX_RELEASE_TIME_def unat_sub MAX_PERIOD_mult)
+
+end
